AwsCryptographicMaterialProviders/dafny/AwsCryptographyKeyStoreAdmin/test/Mutations/TestMutationHappyPath.dfy
@@ -308,8 +308,8 @@ module {:options "/functionSyntax:4" } TestMutationHappyPath {
     expect Structure.BranchKeyContext?(actualEC),
       "Actual EC is not a branch key context. It might not contain restricted keys.";
     if (expectedHV == "2") {
-      expect HvUtils.HasUniqueTransformedKeys?(actualEC),
-        "Actual EC does not have unique transformed keys.";
+      expect HvUtils.IsValidHV2EC?(actualEC),
+        "Actual EC is invalid and is prefixed with 'aws-crypto-ec'";
       expect HvUtils.SelectKmsEncryptionContextForHv2(actualEC) == expectedCustomEC,
         "Actual customer send EC and expected customer send EC did not match.";
     }
